src/core/bir_typing_progScript.sml
@@ -12,16 +12,26 @@ val _ = new_theory "bir_typing_prog";
 (*  Programs                                                                 *)
 (* ------------------------------------------------------------------------- *)
 
+val bir_is_well_typed_label_exp_def = Define `
+  (bir_is_well_typed_label_exp (BLE_Label _) = T) /\
+  (bir_is_well_typed_label_exp (BLE_Exp e) = (case (type_of_bir_exp e) of
+      NONE => F
+    | SOME ty => (bir_type_is_Imm ty)))`;
+
 val bir_is_well_typed_stmtE_def = Define `
-  (bir_is_well_typed_stmtE (BStmt_Jmp _) = T) /\
-  (bir_is_well_typed_stmtE (BStmt_CJmp c _ _) = (type_of_bir_exp c = SOME BType_Bool)) /\
+  (bir_is_well_typed_stmtE (BStmt_Jmp le) = bir_is_well_typed_label_exp le) /\
+  (bir_is_well_typed_stmtE (BStmt_CJmp c le1 le2) = 
+       (type_of_bir_exp c = SOME BType_Bool) /\
+       (bir_is_well_typed_label_exp le1) /\
+       (bir_is_well_typed_label_exp le2)) /\
   (bir_is_well_typed_stmtE (BStmt_Halt e) = (type_of_bir_exp e <> NONE))`
 
 val bir_is_well_typed_stmtB_def = Define `
   (bir_is_well_typed_stmtB (BStmt_Declare _) = T) /\
   (bir_is_well_typed_stmtB (BStmt_Assign v e) = (type_of_bir_exp e = SOME (bir_var_type v))) /\
   (bir_is_well_typed_stmtB (BStmt_Assert e) = (type_of_bir_exp e = SOME BType_Bool)) /\
-  (bir_is_well_typed_stmtB (BStmt_Assume e) = (type_of_bir_exp e = SOME BType_Bool))`;
+  (bir_is_well_typed_stmtB (BStmt_Assume e) = (type_of_bir_exp e = SOME BType_Bool)) /\
+  (bir_is_well_typed_stmtB (BStmt_Observe e _ _) = (type_of_bir_exp e = SOME BType_Bool))`;
 
 val bir_is_well_typed_stmt_def = Define `
   (bir_is_well_typed_stmt (BStmtE s) = bir_is_well_typed_stmtE s) /\
